Changed Nat in auto defs into Type with DecidableEq

lean4/Automaton/DFA/ToNFA.lean
@@ -13,17 +13,17 @@ open DFA NFA
 
 namespace ToNFA
 
-variable {σ : Type _} (td sd : DFA σ) (tn sn : NFA σ)
+variable {α : Type _} {σ : Type _} [DecidableEq α] (td sd : DFA α σ) (tn sn : NFA α σ)
 
 -- dfa and nfa accept the same language
 def dfa_nfa_eq : Prop := ∀ w : word σ , nfa_accepts tn w ↔ dfa_accepts td w
 
 -- to convert into nfa δ, just create singleton for each state
-def dfa_δ_to_nfa_δ : Nat → σ → Finset Nat := λ q e => {td.δ q e}
+def dfa_δ_to_nfa_δ : α → σ → Finset α := λ q e => {td.δ q e}
 
 -- conversion from nfa to dfa
-def dfa_to_nfa : NFA σ := by
-  exact {q := td.q , init := td.init , fs := td.fs , δ := dfa_δ_to_nfa_δ td : NFA σ}
+def dfa_to_nfa : NFA α σ := by
+  exact {q := td.q , init := td.init , fs := td.fs , δ := dfa_δ_to_nfa_δ td : NFA α σ}
 
 -- the initial state in NFA is same as in the original DFA
 theorem dfa_to_nfa_eq_init : td.init = (dfa_to_nfa td).init := by dsimp [dfa_to_nfa]
@@ -37,7 +37,7 @@ theorem dfa_to_nfa_eq_δ_star  (w : word σ) : {DFA.δ_star td w} = NFA.δ_star 
   | nil => dsimp [DFA.δ_star,NFA.δ_star]; rw [←dfa_to_nfa_eq_init]
   | cons a as h => dsimp [DFA.δ_star,NFA.δ_star] 
                    rw [←h];
-                   simp [δ_step,dfa_to_nfa,dfa_δ_to_nfa_δ, δ']              
+                   simp [δ_step,dfa_to_nfa,dfa_δ_to_nfa_δ]              
 
 -- converted dfa accepts the same language as the original dfa
 theorem dfa_to_nfa_eq : dfa_nfa_eq td (dfa_to_nfa td) := by
