lean4/Automaton/NFA/ToDFA.lean
@@ -6,22 +6,19 @@ open NFA DFA
 
 namespace ToDFA
 
-variable {σ : Type _} (tn : NFA σ) (td : DFA σ )
+variable {α : Type _}{σ : Type _} [DecidableEq α] (tn : NFA α σ)
 
 -- turn nfa function into dfa
-def nfa_δ_to_dfa_δ : Finset Nat → σ → Finset Nat := by
+def nfa_δ_to_dfa_δ : Finset α → σ → Finset α := by
   intro q e
   exact q.biUnion (fun n => tn.δ n e)
 
 -- δ_star for converted dfa
-def δ_star (w : word σ) : Finset (Finset Nat) := by
+def δ_star (w : word σ) : Finset (Finset α) := by
   induction w with
   | nil => exact {{tn.init}}
   | cons e _ s => exact s.biUnion (fun n => {(nfa_δ_to_dfa_δ tn) n e})
 
 -- the final state are all sets of states that include at least one final state
-def fs : Finset (Finset Nat) := by
+def fs : Finset (Finset α) := by
   exact (Finset.powerset tn.q).filter (fun q => (q ∩ tn.fs).Nonempty) 
-
-
-end ToDFA
